define typing for instructions; int and bool now no longer import any of the outdated def.s

theories/typing/programs.v
@@ -1,24 +1,30 @@
-From iris.program_logic Require Import hoare.
 From iris.base_logic Require Import big_op.
 From lrust.lang Require Export notation memcpy.
-From lrust.typing Require Export type.
-From lrust.typing Require Import perm lft_contexts type_context cont_context.
 From lrust.lang Require Import proofmode.
 From lrust.lifetime Require Import frac_borrow reborrow borrow creation.
+From lrust.typing Require Export type lft_contexts type_context cont_context.
 
 Section typing.
   Context `{typeG Σ}.
 
+  (** Function Body *)
   Definition typed_body (E : elctx) (L : llctx) (C : cctx) (T : tctx)
                         (e : expr) : iProp Σ :=
     (∀ tid qE, lft_ctx -∗ elctx_interp E qE -∗ llctx_interp L 1 -∗
                (elctx_interp E qE -∗ cctx_interp tid C) -∗ tctx_interp tid T -∗
                WP e {{ _, cont_postcondition }})%I.
+  Global Arguments typed_body _ _ _ _ _%E.
 
   Instance typed_body_llctx_permut E :
     Proper ((≡ₚ) ==> eq ==> eq ==> eq ==> (⊢)) (typed_body E).
   Proof.
     intros L1 L2 HL C ? <- T ? <- e ? <-. rewrite /typed_body. by setoid_rewrite HL.
+  Qed.
+
+  Instance typed_body_elctx_permut :
+    Proper ((≡ₚ) ==> eq ==> eq ==> eq ==> eq ==> (⊢)) typed_body.
+  Proof.
+    intros E1 E2 HE L ? <- C ? <- T ? <- e ? <-. rewrite /typed_body. by setoid_rewrite HE.
   Qed.
 
   Instance typed_body_mono E L:
@@ -31,4 +37,12 @@ Section typing.
     iIntros "HE". by iApply (HC with "LFT HC").
   Qed.
 
+  (** Instruction *)
+  Definition typed_instruction (E : elctx) (L : llctx)
+             (T1 : tctx) (e : expr) (T2 : val → tctx) : iProp Σ :=
+    (∀ tid qE, □ (lft_ctx -∗ elctx_interp E qE -∗ llctx_interp L 1 -∗ tctx_interp tid T1 -∗
+                   WP e {{ v, elctx_interp E qE ∗ llctx_interp L 1 ∗ tctx_interp tid (T2 v) }}))%I.
+  Global Arguments typed_instruction _ _ _ _%E _.
 End typing.
+
+Notation typed_instruction_ty E L T1 e ty := (typed_instruction E L T1 e (λ v : val, [TCtx_hasty v ty])).
